ntt spec in progress, halfway with conv theorem

code/mlkem/Hacl.Spec.MLkem.NTT.fst
@@ -6,283 +6,845 @@ unfold let max = FStar.Math.Lib.max
 open Lib.IntTypes
 open Lib.Sequence
 open Lib.NatMod
+module Fermat = FStar.Math.Fermat
+module Euclid = FStar.Math.Euclid
+module ML = FStar.Math.Lemmas
 open Hacl.Spec.MLkem.Poly
+open Hacl.Spec.MLkem.Zq
+open Hacl.Spec.MLkem.Sums
+open Hacl.Spec.MLkem.PowModInt
+open Hacl.Spec.MLkem.Unity
 
-#reset-options "--z3rlimit 50 --fuel 0 --ifuel 0"
+#reset-options "--z3rlimit 10 --fuel 0 --ifuel 0"
 
-let zeta = 17
-let bit7 = lseq bool 7
+// let bit7 = lseq bool 7
 
-let bitrev7 (bits:bit7): bit7 =
-  createi 7 (fun i -> index bits (6 - i))
+// let bitrev7 (bits:bit7): bit7 =
+//   createi 7 (fun i -> index bits (6 - i))
 
-let bit (b:bool): b:nat{b = 0 || b = 1} = if b then 1 else 0
+// let bit (b:bool): b:nat{b = 0 || b = 1} = if b then 1 else 0
 
-let bit7_v (bits:bit7): r:nat{r < 128} =
-  let r0 = bit (index bits 0) in 
-  let r1 = bit (index bits 1) in
-  let r2 = bit (index bits 2) in
-  let r3 = bit (index bits 3) in
-  let r4 = bit (index bits 4) in
-  let r5 = bit (index bits 5) in
-  let r6 = bit (index bits 6) in
-  r0 + 2 * r1 + 4 * r2 + 8 * r3 + 16 * r4 + 32 * r5 + 64 * r6
+// let bit7_v (bits:bit7): r:nat{r < 128} =
+//   let r0 = bit (index bits 0) in 
+//   let r1 = bit (index bits 1) in
+//   let r2 = bit (index bits 2) in
+//   let r3 = bit (index bits 3) in
+//   let r4 = bit (index bits 4) in
+//   let r5 = bit (index bits 5) in
+//   let r6 = bit (index bits 6) in
+//   r0 + 2 * r1 + 4 * r2 + 8 * r3 + 16 * r4 + 32 * r5 + 64 * r6
 
-let bitrev_ok (bits:bit7): Lemma 
-  (requires True) 
-  (ensures (
-    let rev = bitrev7 bits in
-    forall (i:nat{ i < 7 }). (index bits i = index rev (6 - i))
-  )) = ()
+// let bitrev_ok (bits:bit7): Lemma 
+//   (requires True) 
+//   (ensures (
+//     let rev = bitrev7 bits in
+//     forall (i:nat{ i < 7 }). (index bits i = index rev (6 - i))
+//   )) = ()
 
-let get_bit (bits:nat{ bits < 128}) (i:nat{i < 7}): b:nat{b = 0 || b = 1 } =
-  bits / (pow2 i) % 2
+// let get_bit (bits:nat{ bits < 128}) (i:nat{i < 7}): b:nat{b = 0 || b = 1 } =
+//   bits / (pow2 i) % 2
 
-let bitsequence (i:nat{ i < 128}): bit7 =
-  createi 7 (fun j -> (get_bit i j) = 1)
+// let bitsequence (i:nat{ i < 128}): bit7 =
+//   createi 7 (fun j -> (get_bit i j) = 1)
 
-let bitrev7_int (bits:nat{bits < 128}): result:nat{result < 128} =
-  bit7_v (bitrev7 (bitsequence bits))
+// let bitrev7_int (bits:nat{bits < 128}): result:nat{result < 128} =
+//   bit7_v (bitrev7 (bitsequence bits))
 
 // Types specifying the possible values of the length and start parameters
 type len_t = l:nat{l = 2 || l = 4 || l = 8 || l = 16 || l = 32 || l = 64 || l = 128}
 type start_t (len:len_t) = s:nat{s % (2*len) = 0 && s < 256}
 
-// These just convert between the two representations of polynomials, such that 
-// f[2i] = p[i][0] and f[2i+1] = p[i][1] (does not do the actual NTT)
-// let rq_to_tq (f:rq): tq =
-//   createi 128 (fun i ->
-//     let f0 = index f (2 * i) in
-//     let f1 = index f (2 * i + 1) in
-//     let p: lpoly 2 = cons f0 (cons f1 empty) in
-//     p
-//   )
-// let tq_to_rq (f:tq): rq =
-//   createi 256 (fun i ->
-//     let p = index f (i / 2) in
-//     if i % 2 = 0 then
-//       index p 0
-//     else
-//       index p 1
-//   )
-// let tq_eq (f g: tq) = 
-//   let f_rq = tq_to_rq f in
-//   let g_rq = tq_to_rq g in
-//   Seq.equal f_rq g_rq
+let psi: primitive_nth_root_of_unity_mod #q 512 =
+  assume (pow_mod #q 799 512 == 1);
+  assume (is_primitive #q #512 799);
+  799
 
-val ntt_inner_inner:
-    z:zq
-  -> f:tq
-  -> j:nat
-  -> len:len_t
-  -> start:start_t len
-  -> Tot (tq) (decreases (start + len) - j)
-let rec ntt_inner_inner z f j len start: tq =
-  // for j <- start; j < start + len; j++
-  if j < (start + len) then
-    // t <- zeta * f_hat[j+ len]
-    let t = mul_zq z (index_tq f (j + len)) in
-    let f_j = index_tq f j in
-    // f_hat[j + len] <- f_hat[j] - t
-    let f_upd = upd_tq f (j + len) (add_zq f_j (neg_zq t)) in
-    // f_hat[j] <- f_hat[j] + t
-    let f_upd_upd = upd_tq f_upd j (add_zq f_j t) in
-    ntt_inner_inner z f_upd_upd (j + 1) len start
+val pow_psi: (n:int) -> zq
+let pow_psi n = pow_mod_int #q psi n
+
+// Lemma: psi^-n, where n is positive, can be rewritten as (psi^(-1))^n (or the modular inverse raised to n)
+val pow_psi_mod_inverse_lemma:
+    n:int{n < 0}
+  -> Lemma (pow_psi n == pow_mod #q (pow_psi (-1)) (-n))
+let pow_psi_mod_inverse_lemma n =
+  assert (pow_psi (-1) == pow_mod #q psi (q - 2));
+  calc (==) {
+    pow_psi n;
+    (==) {}
+    pow_mod #q psi ((-n) * (q - 2));
+    (==) {lemma_pow_mod #q psi ((-n) * (q - 2))}
+    pow psi ((-n) * (q - 2)) % q;
+    (==) {lemma_pow_mul psi (q - 2) (-n)}
+    pow (pow psi (q - 2)) (-n) % q;
+    (==) {lemma_pow_mod_base (pow psi (q - 2)) (-n) q}
+    pow (pow psi (q - 2) % q) (-n) % q;
+    (==) {lemma_pow_mod #q psi (q - 2)}
+    pow (pow_mod #q psi (q - 2)) (-n) % q;
+    (==) {}
+    pow (pow_psi (-1)) (-n) % q;
+    (==) {lemma_pow_mod (pow_psi (-1)) (-n)}
+    pow_mod #q (pow_psi (-1)) (-n);
+  }
+  
+val lemma_pow_psi_identity_: (n:nat) -> Lemma (requires True) (ensures (pow_psi n %* pow_psi (-n) == 1))
+let lemma_pow_psi_identity_ n = 
+  Fermat.fermat_alt q psi;
+  calc (==) {
+    pow_psi n %* pow_psi (-n);
+    (==) {}
+    pow_mod #q psi n %* pow_mod #q psi (n * (q - 2));
+    (==) {lemma_pow_mod #q psi n; lemma_pow_mod #q psi (n * (q - 2))}
+    (pow psi n % q) %* (pow psi (n * (q - 2)) % q);
+    (==) {}
+    (pow psi n % q) * (pow psi (n * (q - 2)) % q) % q;
+    (==) {ML.lemma_mod_mul_distr_r (pow psi n) (pow psi (n * (q - 2))) q;
+          ML.lemma_mod_mul_distr_l (pow psi n) (pow psi (n * (q - 2)) % q) q}
+    (pow psi n) * (pow psi (n * (q - 2))) % q;
+    (==) {lemma_pow_add psi n (n * (q - 2))}
+    (pow psi (n + n * (q - 2))) % q;
+    (==) {}
+    (pow psi ((q - 1) * n)) % q;
+    (==) {lemma_pow_mul psi (q - 1) n; lemma_pow_eq_fermat_pow psi (q - 1)}
+    (pow (Fermat.pow psi (q - 1)) n) % q;
+    (==) {lemma_pow_mod_base (Fermat.pow psi (q-1)) n q}
+    (pow 1 n) % q;
+    (==) {lemma_pow_one n}
+    1 % q;
+  }
+
+val lemma_pow_psi_identity: (n:int) -> Lemma (requires True) (ensures (pow_psi n %* pow_psi (-n) == 1))
+let lemma_pow_psi_identity n =
+  if n >= 0 then 
+    lemma_pow_psi_identity_ n
   else
-    f
+    lemma_pow_psi_identity_ (-n)
 
-val ntt_inner_inner_f (j:nat{j < 256}) (len:len_t) (start:start_t len) (z:zq) (f:tq): zq
-let ntt_inner_inner_f j len start z f =
-    if j < start || j >= start + 2 * len then
-      index_tq f j
-    else if j >= start && j < start + len then
-      let t = mul_zq z (index_tq f (j + len)) in
-      add_zq (index_tq f j) t
-    else
-      let t = mul_zq z (index_tq f j) in
-      add_zq (index_tq f (j - len)) (neg_zq t)
+// let pow_mod_int_neg_one (n:int): zq =
+//   // pow_mod #q (neg_zq 1) (int_to_zq n)
+//   if n % 2 = 0 then 1 else ((-1) % q)
+
+val lemma_rewrite_pow_psi_conv_theorem:
+    i:int
+  -> j:int 
+  -> k:int
+  -> Lemma (pow_mod_int_neg_one ((i - j) / n) %* pow_psi ((i - j) * (2 * k + 1))
+         == pow_psi ((i - j % n) * (2 * k + 1)))
+let lemma_rewrite_pow_psi_conv_theorem i j k = admit()
+
+val mul_quotient_ring_kth_term:
+    f:rq
+  -> g:rq
+  -> k:int
+  -> zq
+let mul_quotient_ring_kth_term f g k =
+  if k < 0 || k >= n then 0
+  else sum_of_zqs 0 n (fun j -> (pow_mod_int_neg_one ((k - j) / n)) %* (f.[j] %* g.[(k - j) % n]))
+
+val mul_quotient_ring:
+    f:rq
+  -> g:rq
+  -> rq
+let mul_quotient_ring f g = 
+  createi n (fun k -> mul_quotient_ring_kth_term f g k)
+
+val mul_quotient_ring_lemma:
+    f:rq
+  -> g:rq
+  -> k:int
+  -> Lemma ((mul_quotient_ring f g).[k] == mul_quotient_ring_kth_term f g k)
+let mul_quotient_ring_lemma f g k = ()
+
+// If we have a polynomial a = a_0 + a_1 * X + a_2 * X^2 + a_3 * X^3 + ... + a_n-1 * X^n-1
+// then the NTT should be  a*_k = sum_{j=0}^{n-1} a_j * omega_n^(j*k),
+// where omega_n is the nth root of unity
+val ntt_kth_term:
+    f:lpoly n
+  -> k:int
+  -> zq
+let ntt_kth_term f k = 
+  if k < 0 || k >= n then 0 
+  else sum_of_zqs 0 n (fun j -> mul_zq (f.[j]) (pow_psi (j * (2 * k + 1))))
+
+val ntt_kth_term_lemma:
+    f:lpoly n
+  -> k:nat{k < n}
+  -> Lemma ((ntt_kth_term f k) == sum_of_zqs 0 n (fun j -> mul_zq (f.[j]) (pow_psi (j * (2 * k + 1)))))
+  [SMTPat (ntt_kth_term f k)] 
+let ntt_kth_term_lemma f k = ()
+
+let ntt (f:lpoly n) =
+  createi n (fun k -> ntt_kth_term f k)
+
+val ntt_lemma (f:lpoly n) (i:int): 
+  Lemma ((ntt f).[i] == ntt_kth_term f i)
+  [SMTPat ((ntt f).[i])]
+let ntt_lemma f i = ()
 
 
-val ntt_inner_inner_func:
-    z:zq 
-  -> f:tq 
-  -> len:len_t
-  -> start:start_t len
-  -> tq
-let ntt_inner_inner_func z f len start = 
-  let rq_rep = createi #zq 256 (fun j -> ntt_inner_inner_f j len start z f) in rq_to_tq rq_rep
+val intt_kth_term:
+    f:lpoly n
+  -> k:int
+  -> zq
+let intt_kth_term f k =
+  if k < 0 || k >= n then 0
+  else sum_of_zqs 0 (n-1) (fun i -> mul_zq (f.[i]) (pow_psi (-k * (2 * i + 1))))
 
-// val ntt_inner_inner_func_ok: 
+let intt (f:lpoly n) = createi n (fun k -> intt_kth_term f k)
+
+val intt_lemma (f:lpoly n) (i:int): 
+  Lemma ((intt f).[i] == intt_kth_term f i)
+  [SMTPat (index (intt f) i)]
+let intt_lemma f i = ()
+
+// INTT(NTT(f))_k
+val intt_ntt_kth_term:
+    f:lpoly n
+  -> k:nat{k < n}
+  -> zq
+let intt_ntt_kth_term f k = 
+  sum_of_zqs 0 (n-1) (fun i -> mul_zq (ntt_kth_term f i) (pow_psi (-k * (2 * i + 1)))) / n
+
+val intt_ntt_is_id_kth_term: 
+    (f:lpoly n) 
+  -> (k:nat{k < n}) 
+  -> Lemma (ensures (f.[k]) == ((intt (ntt f)).[k]))
+let intt_ntt_is_id_kth_term f k =
+  let rhs = intt_ntt_kth_term f k in
+  assert (rhs == sum_of_zqs 0 (n-1) (fun i -> mul_zq (ntt_kth_term f i) (pow_psi (-k * (2 * i + 1)))) / n);
+  admit()
+
+val intt_ntt_is_id:
+    f:rq
+  -> Lemma (requires True) (ensures Seq.equal f (intt (ntt f)))
+let intt_ntt_is_id f =
+  admit()
+
+
+val ntt_intt_is_id:
+    f:rq
+  -> Lemma (requires True) (ensures Seq.equal f (ntt (intt f)))
+let ntt_intt_is_id f =
+  admit()
+
+
+let mul_componentwise (f g:rq) = createi n (fun i -> f.[i] %* g.[i])
+
+val convolution_theorem_kth_term_ok_1:
+    f:rq
+  -> g:rq
+  -> k:nat{k < n}
+  -> Lemma 
+      (requires True) 
+      (ensures ntt_kth_term (mul_quotient_ring f g) k 
+            == sum_of_zqs 0 n (fun i -> (sum_of_zqs 0 n (fun j -> pow_psi (i * (2 * k + 1)) %* (pow_mod_int_neg_one ((i - j) / n)) %* (f.[j] %* g.[(i - j) % n])))))
+let convolution_theorem_kth_term_ok_1 f g k =
+  ntt_kth_term_lemma (mul_quotient_ring f g) k;
+  let lhs_inner_f = (fun i -> (mul_quotient_ring f g).[i] %* pow_psi (i * (2 * k + 1))) in
+  let lhs_inner_f' = (fun i -> pow_psi (i * (2 * k + 1)) %* (sum_of_zqs 0 n (fun j -> (pow_mod_int_neg_one ((i - j) / n)) %* (f.[j] %* g.[(i - j) % n])))) in
+  let f_i = fun i -> pow_psi (i * (2 * k + 1)) in
+  let f_j = fun i j -> (pow_mod_int_neg_one ((i - j) / n)) %* (f.[j] %* g.[(i - j) % n]) in
+  sum_rewrite_lemma 0 n lhs_inner_f lhs_inner_f';
+  double_sum_mul_lemma 0 n 0 n f_i f_j
+  
+val convolution_theorem_kth_term_ok_2:
+    f:rq
+  -> g:rq
+  -> k:nat{k < n}
+  -> Lemma 
+      (requires True) 
+      (ensures ntt_kth_term (mul_quotient_ring f g) k
+            == sum_of_zqs 0 n (fun j -> (sum_of_zqs 0 n (fun i -> pow_psi (i * (2 * k + 1)) %* (pow_mod_int_neg_one ((i - j) / n)) %* f.[j] %* g.[(i - j) % n]))))
+let convolution_theorem_kth_term_ok_2 f g k =
+  convolution_theorem_kth_term_ok_1 f g k;
+  swap_sum_order 0 n 0 n (fun i j -> pow_psi (i * (2 * k + 1)) %* (pow_mod_int_neg_one ((i - j) / n)) %* (f.[j] %* g.[(i - j) % n]))
+
+#reset-options "--z3rlimit 20 --fuel 0 --ifuel 0"
+val convolution_theorem_kth_term_ok_3_:
+    f:rq 
+  -> g:rq
+  -> k:nat{k < n}
+  -> Lemma 
+      (requires True) 
+      (ensures ntt_kth_term (mul_quotient_ring f g) k
+            == sum_of_zqs 0 n (fun j -> (sum_of_zqs 0 n (fun i -> f.[j] %* pow_psi (i * (2 * k + 1)) %* (pow_mod_int_neg_one ((i - j) / n)) %* g.[(i - j) % n])))
+      )
+let convolution_theorem_kth_term_ok_3_ f g k =
+  convolution_theorem_kth_term_ok_2 f g k;
+  // First step is to rearrange the terms in the inner sum so that we can apply our sum multiplication lemma
+  let original = (fun j -> (sum_of_zqs 0 n (fun i -> pow_psi (i * (2 * k + 1)) %* (pow_mod_int_neg_one ((i - j) / n)) %* f.[j] %* g.[(i - j) % n]))) in
+  let original' = (fun j -> (sum_of_zqs 0 n (fun i -> f.[j] %* pow_psi (i * (2 * k + 1)) %* (pow_mod_int_neg_one ((i - j) / n)) %* g.[(i - j) % n]))) in
+  let lemma_aux (j:int): Lemma (ensures (original j == original' j)) =
+    let first = (fun i -> pow_psi (i * (2 * k + 1)) %* (pow_mod_int_neg_one ((i - j) / n)) %* f.[j] %* g.[(i - j) % n]) in
+    let second = (fun i -> f.[j] %* pow_psi (i * (2 * k + 1)) %* (pow_mod_int_neg_one ((i - j) / n)) %* g.[(i - j) % n]) in
+    let lemma_aux' (i:int): Lemma (ensures (first i == second i)) =
+      lemma_mul_rearrange (pow_psi (i * (2 * k + 1))) (pow_mod_int_neg_one ((i - j) / n)) f.[j] g.[(i - j) % n] in
+    Classical.forall_intro (lemma_aux') in
+  Classical.forall_intro (lemma_aux);
+  sum_rewrite_lemma 0 n original original'
+
+val convolution_theorem_kth_term_ok_3:
+  f:rq 
+  -> g:rq
+  -> k:nat{k < n}
+  -> Lemma 
+      (requires True) 
+      (ensures ntt_kth_term (mul_quotient_ring f g) k
+            == sum_of_zqs 0 n (fun j -> f.[j] %* (sum_of_zqs 0 n (fun i -> pow_psi (i * (2 * k + 1)) %* (pow_mod_int_neg_one ((i - j) / n)) %* g.[(i - j) % n]))))
+let convolution_theorem_kth_term_ok_3 f g k =
+  convolution_theorem_kth_term_ok_3_ f g k;
+  // First step is to rearrange the terms in the inner sum so that we can apply our sum multiplication lemma
+  let original' = (fun j -> (sum_of_zqs 0 n (fun i -> f.[j] %* pow_psi (i * (2 * k + 1)) %* (pow_mod_int_neg_one ((i - j) / n)) %* g.[(i - j) % n]))) in
+  // Next step is to apply the sum multiplication lemma, and then we need to do an additional small step to remove the parenthesization
+  let goal = (fun j -> f.[j] %* (sum_of_zqs 0 n (fun i -> pow_psi (i * (2 * k + 1)) %* (pow_mod_int_neg_one ((i - j) / n)) %* g.[(i - j) % n]))) in
+  let lemma_aux2 (j:int): Lemma (ensures original' j == goal j) =
+    sum_mul_lemma f.[j] 0 n (fun i -> pow_psi (i * (2 * k + 1)) %* (pow_mod_int_neg_one ((i - j) / n)) %* g.[(i - j) % n]);
+    let parenthesized = (fun i -> f.[j] %* (pow_psi (i * (2 * k + 1)) %* (pow_mod_int_neg_one ((i - j) / n)) %* g.[(i - j) % n])) in
+    let unparenthesized = (fun i -> f.[j] %* pow_psi (i * (2 * k + 1)) %* (pow_mod_int_neg_one ((i - j) / n)) %* g.[(i - j) % n]) in
+    let lemma_aux2' (i:int): Lemma (ensures (parenthesized i == unparenthesized i)) =
+      lemma_mul_assoc_big f.[j] (pow_psi (i * (2 * k + 1))) (pow_mod_int_neg_one ((i - j) / n)) g.[(i - j) % n] in
+    Classical.forall_intro (lemma_aux2') in
+  Classical.forall_intro (lemma_aux2);
+  sum_rewrite_lemma 0 n original' goal
+
+
+val convolution_theorem_kth_term_ok_4_:
+    f:rq 
+  -> g:rq
+  -> k:nat{k < n}
+  -> j:int
+  -> i:int
+  -> Lemma 
+      (requires True) 
+      (ensures pow_psi (i * (2 * k + 1)) %* (pow_mod_int_neg_one ((i - j) / n)) %* g.[(i - j) % n]
+            == pow_psi (j * (2 * k + 1)) %* pow_psi (i * (2 * k + 1)) %* pow_psi (-j * (2 * k + 1)) %* (pow_mod_int_neg_one ((i - j) / n)) %* g.[(i - j) % n]
+      )
+let convolution_theorem_kth_term_ok_4_ f g k j i =
+  lemma_pow_psi_identity (j * (2 * k + 1));
+  assert (pow_psi (j * (2 * k + 1)) %* pow_psi (-j * (2 * k + 1)) == 1);
+  calc (==) {
+    pow_psi (i * (2 * k + 1)) %* (pow_mod_int_neg_one ((i - j) / n)) %* g.[(i - j) % n];
+    (==) {}
+    pow_psi (i * (2 * k + 1)) %* 1 %* (pow_mod_int_neg_one ((i - j) / n)) %* g.[(i - j) % n];
+    (==) {}
+    pow_psi (i * (2 * k + 1)) %* (pow_psi (j * (2 * k + 1)) %* pow_psi (-j * (2 * k + 1))) %* (pow_mod_int_neg_one ((i - j) / n)) %* g.[(i - j) % n];
+    (==) {}
+    pow_psi (i * (2 * k + 1)) %* pow_psi (j * (2 * k + 1)) %* pow_psi (-j * (2 * k + 1)) %* (pow_mod_int_neg_one ((i - j) / n)) %* g.[(i - j) % n];
+    (==) {}
+    pow_psi (j * (2 * k + 1)) %* pow_psi (i * (2 * k + 1)) %* pow_psi (-j * (2 * k + 1)) %* (pow_mod_int_neg_one ((i - j) / n)) %* g.[(i - j) % n];
+  }
+
+val convolution_theorem_kth_term_ok_4_aux_:
+    f:rq 
+  -> g:rq
+  -> k:nat{k < n}
+  -> j:int
+  -> Lemma 
+      (requires True) 
+      (ensures (sum_of_zqs 0 n (fun i -> pow_psi (i * (2 * k + 1)) %* (pow_mod_int_neg_one ((i - j) / n)) %* g.[(i - j) % n]))
+            == (sum_of_zqs 0 n (fun i -> pow_psi (j * (2 * k + 1)) %* pow_psi (i * (2 * k + 1)) %* pow_psi (-j * (2 * k + 1)) %* (pow_mod_int_neg_one ((i - j) / n)) %* g.[(i - j) % n])))
+let convolution_theorem_kth_term_ok_4_aux_ f g k j =
+  let original = (fun i -> pow_psi (i * (2 * k + 1)) %* (pow_mod_int_neg_one ((i - j) / n)) %* g.[(i - j) % n]) in
+  let goal = (fun i -> pow_psi (j * (2 * k + 1)) %* pow_psi (i * (2 * k + 1)) %* pow_psi (-j * (2 * k + 1)) %* (pow_mod_int_neg_one ((i - j) / n)) %* g.[(i - j) % n]) in
+  Classical.forall_intro (convolution_theorem_kth_term_ok_4_ f g k j)
+
+val convolution_theorem_kth_term_ok_4_aux:
+    f:rq 
+  -> g:rq
+  -> k:nat{k < n}
+  -> j:int
+  -> Lemma 
+      (requires True) 
+      (ensures f.[j] %* (sum_of_zqs 0 n (fun i -> pow_psi (i * (2 * k + 1)) %* (pow_mod_int_neg_one ((i - j) / n)) %* g.[(i - j) % n]))
+            == f.[j] %* (sum_of_zqs 0 n (fun i -> pow_psi (j * (2 * k + 1)) %* pow_psi (i * (2 * k + 1)) %* pow_psi (-j * (2 * k + 1)) %* (pow_mod_int_neg_one ((i - j) / n)) %* g.[(i - j) % n])))
+let convolution_theorem_kth_term_ok_4_aux f g k j =
+  convolution_theorem_kth_term_ok_4_aux_ f g k j
+
+// Adds pow_psi (j * (2 * k + 1)) %* pow_psi (-j * (2 * k + 1)) = 1 into the inner sum
+val convolution_theorem_kth_term_ok_4:
+    f:rq 
+  -> g:rq
+  -> k:nat{k < n}
+  -> Lemma 
+      (requires True) 
+      (ensures ntt_kth_term (mul_quotient_ring f g) k
+            == sum_of_zqs 0 n (fun j -> f.[j] %* (sum_of_zqs 0 n (fun i -> pow_psi (j * (2 * k + 1)) %* pow_psi (i * (2 * k + 1)) %* pow_psi (-j * (2 * k + 1)) %* (pow_mod_int_neg_one ((i - j) / n)) %* (g.[(i - j) % n])))))
+let convolution_theorem_kth_term_ok_4 f g k =
+  convolution_theorem_kth_term_ok_3 f g k;
+  Classical.forall_intro (convolution_theorem_kth_term_ok_4_aux f g k)
+
+val convolution_theorem_kth_term_ok_5_aux_:
+    f:rq 
+  -> g:rq
+  -> k:nat{k < n}
+  -> j:int
+
+  -> Lemma 
+      (requires True) 
+      (ensures (sum_of_zqs 0 n (fun i -> pow_psi (j * (2 * k + 1)) %* pow_psi (i * (2 * k + 1)) %* pow_psi (-j * (2 * k + 1)) %* (pow_mod_int_neg_one ((i - j) / n)) %* (g.[(i - j) % n])))
+            == pow_psi (j * (2 * k + 1)) %* (sum_of_zqs 0 n (fun i -> pow_psi (i * (2 * k + 1)) %* pow_psi (-j * (2 * k + 1)) %* (pow_mod_int_neg_one ((i - j) / n)) %* (g.[(i - j) % n]))))
+let convolution_theorem_kth_term_ok_5_aux_ f g k j =
+  let lemma_aux (i:int): Lemma (pow_psi (j * (2 * k + 1)) %* (pow_psi (i * (2 * k + 1)) %* pow_psi (-j * (2 * k + 1)) %* (pow_mod_int_neg_one ((i - j) / n)) %* (g.[(i - j) % n]))
+                             == pow_psi (j * (2 * k + 1)) %* pow_psi (i * (2 * k + 1)) %* pow_psi (-j * (2 * k + 1)) %* (pow_mod_int_neg_one ((i - j) / n)) %* (g.[(i - j) % n])) = 
+    lemma_mul_assoc_bigger (pow_psi (j * (2 * k + 1))) (pow_psi (i * (2 * k + 1))) (pow_psi (-j * (2 * k + 1))) (pow_mod_int_neg_one ((i - j) / n)) (g.[(i - j) % n]) in
+  Classical.forall_intro lemma_aux;
+  sum_mul_lemma (pow_psi (j * (2 * k + 1))) 0 n (fun i -> pow_psi (i * (2 * k + 1)) %* pow_psi (-j * (2 * k + 1)) %* (pow_mod_int_neg_one ((i - j) / n)) %* (g.[(i - j) % n]))
+
+val convolution_theorem_kth_term_ok_5_aux:
+    f:rq 
+  -> g:rq
+  -> k:nat{k < n}
+  -> j:int
+  -> Lemma 
+      (requires True) 
+      (ensures f.[j] %* (sum_of_zqs 0 n (fun i -> pow_psi (i * (2 * k + 1)) %* pow_psi (j * (2 * k + 1)) %* pow_psi (-j * (2 * k + 1)) %* (pow_mod_int_neg_one ((i - j) / n)) %* (g.[(i - j) % n])))
+            == f.[j] %* pow_psi (j * (2 * k + 1)) %* (sum_of_zqs 0 n (fun i -> pow_psi (i * (2 * k + 1)) %* pow_psi (-j * (2 * k + 1)) %* (pow_mod_int_neg_one ((i - j) / n)) %* (g.[(i - j) % n]))))
+let convolution_theorem_kth_term_ok_5_aux f g k j =
+  convolution_theorem_kth_term_ok_5_aux_ f g k j
+
+#reset-options "--z3rlimit 15 --fuel 0 --ifuel 0 --split_queries always"
+// Moves pow_psi (j * (2 * k + 1)) out of the inner sum
+val convolution_theorem_kth_term_ok_5:
+    f:rq 
+  -> g:rq
+  -> k:nat{k < n}
+  -> Lemma 
+      (requires True) 
+      (ensures ntt_kth_term (mul_quotient_ring f g) k
+            == sum_of_zqs 0 n (fun j -> f.[j] %* pow_psi (j * (2 * k + 1)) %* (sum_of_zqs 0 n (fun i -> pow_psi (i * (2 * k + 1)) %* pow_psi (-j * (2 * k + 1)) %* (pow_mod_int_neg_one ((i - j) / n)) %* (g.[(i - j) % n])))))
+let convolution_theorem_kth_term_ok_5 f g k =
+  convolution_theorem_kth_term_ok_4 f g k;
+  assert (ntt_kth_term (mul_quotient_ring f g) k == sum_of_zqs 0 n (fun j -> f.[j] %* (sum_of_zqs 0 n (fun i -> pow_psi (i * (2 * k + 1)) %* pow_psi (j * (2 * k + 1)) %* pow_psi (-j * (2 * k + 1)) %* (pow_mod_int_neg_one ((i - j) / n)) %* (g.[(i - j) % n])))));
+  Classical.forall_intro (convolution_theorem_kth_term_ok_5_aux f g k);
+  assert (ntt_kth_term (mul_quotient_ring f g) k == sum_of_zqs 0 n (fun j -> f.[j] %* pow_psi (j * (2 * k + 1)) %* (sum_of_zqs 0 n (fun i -> pow_psi (i * (2 * k + 1)) %* pow_psi (-j * (2 * k + 1)) %* (pow_mod_int_neg_one ((i - j) / n)) %* (g.[(i - j) % n])))))
+
+#reset-options "--z3rlimit 15 --fuel 1 --ifuel 0"
+val convolution_theorem_kth_term_ok_6_aux_aux_rewrite:
+    f:rq 
+  -> g:rq
+  -> k:nat
+  -> j:int
+  -> i:int
+  -> Lemma (pow_psi (i * (2 * k + 1)) %* pow_psi (-j * (2 * k + 1)) %* (pow_mod_int_neg_one ((i - j) / n)) %* (g.[(i - j) % n])
+         == pow_psi ((i - j) * (2*k+1)) %* (pow_mod_int_neg_one ((i - j) / n)) %* (g.[(i - j) % n]))
+let convolution_theorem_kth_term_ok_6_aux_aux_rewrite f g k j i =
+  calc (==) {
+    pow_psi (i * (2 * k + 1)) %* pow_psi (-j * (2 * k + 1)) %* (pow_mod_int_neg_one ((i - j) / n)) %* (g.[(i - j) % n]);
+    (==) {}
+    (pow_psi (i * (2 * k + 1)) %* pow_psi (-j * (2 * k + 1))) %* (pow_mod_int_neg_one ((i - j) / n)) %* (g.[(i - j) % n]);
+    (==) {lemma_pow_mod_int_add #q psi (i * (2 * k + 1)) (-j * (2 * k + 1))}
+    (pow_psi ((i - j) * (2 * k + 1))) %* (pow_mod_int_neg_one ((i - j) / n)) %* (g.[(i - j) % n]);
+    (==) {}
+    (pow_psi ((i - j) * (2 * k + 1))) %* (pow_mod_int_neg_one ((i - j) / n)) %* (g.[(i - j) % n]);
+  }
+
+val rearrange_6_aux_aux:
+  a:int 
+  -> b:int 
+  -> c:int
+  -> Lemma ((a * b) * c == b * (c * a))
+let rearrange_6_aux_aux a b c = ()
+
+val convolution_theorem_kth_term_ok_6_rewrite:
+    f:rq 
+  -> g:rq
+  -> k:nat
+  -> j:int
+  -> i:int
+  -> Lemma (pow_psi ((i - j) * (2 * k + 1)) %* (pow_mod_int_neg_one ((i - j) / n))
+         == pow_psi (((i - j) % n) * (2 * k + 1)))
+let convolution_theorem_kth_term_ok_6_rewrite f g k j i = 
+  let quot = (i - j) / n in 
+  let r = (i - j) % n in 
+  assert (i - j == quot * n + r);
+  calc (==) {
+    pow_psi ((quot * n + r) * (2 * k + 1)) %* (pow_mod_int_neg_one (quot));
+    (==) {ML.distributivity_add_left (quot * n) r (2 * k + 1)}
+    pow_psi ((quot * n) * (2 * k + 1) + r * (2 * k + 1)) %* (pow_mod_int_neg_one (quot));
+    (==) {lemma_pow_mod_int_add #q psi (quot * n * (2 * k + 1)) (r * (2 * k + 1))}
+    pow_psi ((quot * n) * (2 * k + 1)) %* pow_psi (r * (2 * k + 1)) %* (pow_mod_int_neg_one (quot));
+    (==) {rearrange_6_aux_aux quot n (2 * k + 1)}
+    pow_psi (n * ((2 * k + 1) * quot)) %* pow_psi (r * (2 * k + 1)) %* (pow_mod_int_neg_one (quot));
+    (==) {lemma_pow_mod_int_mul #q psi n ((2 * k + 1) * quot)}
+    pow_mod_int #q (pow_psi n) ((2 * k + 1) * quot) %* pow_psi (r * (2 * k + 1)) %* (pow_mod_int_neg_one (quot));
+    (==) {lemma_primitive_unity_half_n #q #(2*n) psi}
+    pow_mod_int #q ((-1) % q) ((2 * k + 1) * quot) %* pow_psi (r * (2 * k + 1)) %* (pow_mod_int_neg_one (quot));
+    (==) {lemma_pow_mod_int_mul #q ((-1) % q) (2 * k + 1) quot}
+    pow_mod_int #q (pow_mod_int #q ((-1) % q) (2 * k + 1)) quot %* pow_psi (r * (2 * k + 1)) %* (pow_mod_int_neg_one (quot));
+    (==) {lemma_pow_mod_neg_one_eq_pow_mod_pos #q (2 * k + 1)}
+    pow_mod_int #q (pow_mod_int_neg_one #q (2 * k + 1)) quot %* pow_psi (r * (2 * k + 1)) %* (pow_mod_int_neg_one (quot));
+    (==) {}
+    pow_mod_int #q ((-1) % q) quot %* pow_psi (r * (2 * k + 1)) %* (pow_mod_int_neg_one (quot));
+    (==) {lemma_pow_mod_neg_one_eq_pow_mod #q quot}
+    pow_mod_int #q ((-1) % q) quot %* pow_psi (r * (2 * k + 1)) %* (pow_mod_int #q ((-1) % q) quot);
+    (==) {lemma_mul_zq_comm (pow_mod_int #q ((-1) % q) quot) (pow_psi (r * (2 * k + 1)))}
+    pow_psi (r * (2 * k + 1)) %* pow_mod_int #q ((-1) % q) (quot) %* pow_mod_int #q ((-1) % q) (quot);
+    (==) {lemma_mul_zq_assoc (pow_psi (r * (2 * k + 1))) (pow_mod_int #q ((-1) % q) (quot)) (pow_mod_int #q ((-1) % q) (quot))}
+    pow_psi (r * (2 * k + 1)) %* (pow_mod_int #q ((-1) % q) (quot) %* pow_mod_int #q ((-1) % q) (quot));
+    (==) {lemma_pow_mod_int_add #q ((-1) % q) quot quot}
+    pow_psi (r * (2 * k + 1)) %* pow_mod_int #q ((-1) % q) (quot + quot);
+    (==) {lemma_pow_mod_neg_one_eq_pow_mod #q (quot + quot)}
+    pow_psi (r * (2 * k + 1)) %* pow_mod_int_neg_one (quot + quot);
+    (==) {}
+    pow_psi (r * (2 * k + 1));
+  }
+
+val convolution_theorem_kth_term_ok_6_inner_sum_aux:
+    f:rq 
+  -> g:rq 
+  -> k:nat{k < n}
+  -> j:int
+  -> i:int 
+  -> Lemma
+      (pow_psi (i * (2 * k + 1)) %* pow_psi (-j * (2 * k + 1)) %* (pow_mod_int_neg_one ((i - j) / n)) %* (g.[(i - j) % n])
+    == pow_psi (((i - j) % n) * (2 * k + 1)) %* (g.[(i - j) % n]))
+let convolution_theorem_kth_term_ok_6_inner_sum_aux f g k j i =
+  calc (==) {
+    pow_psi (i * (2 * k + 1)) %* pow_psi (-j * (2 * k + 1)) %* (pow_mod_int_neg_one ((i - j) / n)) %* (g.[(i - j) % n]);
+    (==) {convolution_theorem_kth_term_ok_6_aux_aux_rewrite f g k j i}
+    pow_psi ((i - j) * (2 * k + 1)) %* (pow_mod_int_neg_one ((i - j) / n)) %* (g.[(i - j) % n]);
+    (==) {}
+    (pow_psi ((i - j) * (2 * k + 1)) %* (pow_mod_int_neg_one ((i - j) / n))) %* (g.[(i - j) % n]);
+    (==) {convolution_theorem_kth_term_ok_6_rewrite f g k j i}
+    (pow_psi (((i - j) % n) * (2 * k + 1))) %* (g.[(i - j) % n]);
+  }
+
+#reset-options "--z3rlimit 5 --fuel 1 --ifuel 0"
+val convolution_theorem_kth_term_ok_6_outer_sum_aux_helper:
+    f:rq 
+  -> g:rq
+  -> k:nat{k < n}
+  -> j:int
+  -> Lemma
+      ((sum_of_zqs 0 n (fun i -> pow_psi (i * (2 * k + 1)) %* pow_psi (-j * (2 * k + 1)) %* (pow_mod_int_neg_one ((i - j) / n)) %* (g.[(i - j) % n])))
+    == (sum_of_zqs 0 n (fun i -> pow_psi (((i - j) % n) * (2 * k + 1)) %* (g.[(i - j) % n]))))
+let convolution_theorem_kth_term_ok_6_outer_sum_aux_helper f g k j =
+  let original = (fun i -> pow_psi (i * (2 * k + 1)) %* pow_psi (-j * (2 * k + 1)) %* (pow_mod_int_neg_one ((i - j) / n)) %* (g.[(i - j) % n])) in
+  let goal = (fun i -> pow_psi (((i - j) % n) * (2 * k + 1)) %* (g.[(i - j) % n])) in
+  Classical.forall_intro (convolution_theorem_kth_term_ok_6_inner_sum_aux f g k j);
+  sum_rewrite_lemma 0 n original goal
+
+
+val convolution_theorem_kth_term_ok_6_outer_sum_aux:
+    f:rq 
+  -> g:rq
+  -> k:nat{k < n}
+  -> j:int
+  -> Lemma
+      (f.[j] %* pow_psi (j * (2 * k + 1)) %* (sum_of_zqs 0 n (fun i -> pow_psi (i * (2 * k + 1)) %* pow_psi (-j * (2 * k + 1)) %* (pow_mod_int_neg_one ((i - j) / n)) %* (g.[(i - j) % n])))
+    == f.[j] %* pow_psi (j * (2 * k + 1)) %* (sum_of_zqs 0 n (fun i -> pow_psi (((i - j) % n) * (2*k+1)) %* (g.[(i - j) % n]))))
+let convolution_theorem_kth_term_ok_6_outer_sum_aux f g k j =
+  let original = (fun i -> pow_psi (i * (2 * k + 1)) %* pow_psi (-j * (2 * k + 1)) %* (pow_mod_int_neg_one ((i - j) / n)) %* (g.[(i - j) % n])) in
+  let goal = (fun i -> pow_psi (((i - j) % n) * (2*k+1)) %* (g.[(i - j) % n])) in
+  Classical.forall_intro (convolution_theorem_kth_term_ok_6_inner_sum_aux f g k j);
+  sum_rewrite_lemma 0 n original goal
+
+#reset-options "--z3rlimit 15 --fuel 0 --ifuel 0"
+val convolution_theorem_kth_term_ok_6:
+    f:rq 
+  -> g:rq
+  -> k:nat{k < n}
+  -> Lemma 
+      (requires True) 
+      (ensures ntt_kth_term (mul_quotient_ring f g) k
+            == sum_of_zqs 0 n (fun j -> f.[j] %* pow_psi (j * (2 * k + 1)) %* (sum_of_zqs 0 n (fun i -> pow_psi (((i - j) % n) * (2*k+1)) %* (g.[(i - j) % n])))))
+let convolution_theorem_kth_term_ok_6 f g k =
+  convolution_theorem_kth_term_ok_5 f g k;
+  Classical.forall_intro (convolution_theorem_kth_term_ok_6_outer_sum_aux f g k)
+
+val convolution_theorem_kth_term_ok_7:
+    f:rq 
+  -> g:rq
+  -> k:nat{k < n}
+  -> Lemma 
+      (requires True) 
+      (ensures ntt_kth_term (mul_quotient_ring f g) k
+            == sum_of_zqs 0 n (fun j -> f.[j] %* pow_psi (j * (2 * k + 1)) %* (sum_of_zqs 0 n (fun i -> pow_psi (i * (2*k+1)) %* (g.[i])))))
+let convolution_theorem_kth_term_ok_7 f g k =
+  admit()
+
+val convolution_theorem_kth_term_ok_8:
+    f:rq 
+  -> g:rq
+  -> k:nat{k < n}
+  -> Lemma 
+      (requires True) 
+      (ensures ntt_kth_term (mul_quotient_ring f g) k
+            == (sum_of_zqs 0 n (fun j -> f.[j] %* pow_psi (j * (2 * k + 1)))) %* (sum_of_zqs 0 n (fun i -> pow_psi (i * (2*k+1)) %* (g.[i]))))
+let convolution_theorem_kth_term_ok_8 f g k =
+  admit()
+
+val convolution_theorem_kth_term_ok_9:
+    f:rq 
+  -> g:rq
+  -> k:nat{k < n}
+  -> Lemma 
+      (requires True) 
+      (ensures ntt_kth_term (mul_quotient_ring f g) k
+            == ntt_kth_term f k %* ntt_kth_term g k)
+let convolution_theorem_kth_term_ok_9 f g k =
+  admit()
+
+#reset-options "--z3rlimit 10 --fuel 0 --ifuel 0"
+val convolution_theorem_kth_term_ok:
+    f:rq
+  -> g:rq
+  -> k:nat
+  -> Lemma 
+      (requires True) 
+      (ensures (ntt_kth_term (mul_quotient_ring f g) k == ntt_kth_term f k %* ntt_kth_term g k))
+let convolution_theorem_kth_term_ok f g k =
+  if 0 <= k && k < n then 
+    convolution_theorem_kth_term_ok_9 f g k
+  else ()
+
+val convolution_theorem:
+    f:rq
+  -> g:rq
+  -> Lemma 
+      (requires True) 
+      (ensures equal 
+        (ntt (mul_quotient_ring f g))
+        (mul_componentwise (ntt f) (ntt g)))
+let convolution_theorem f g =
+  Classical.forall_intro (convolution_theorem_kth_term_ok f g);
+  let lhs = ntt (mul_quotient_ring f g) in
+  let rhs = mul_componentwise (ntt f) (ntt g) in
+  // assert (forall (i:nat{i < n}).{:pattern (lhs.[i])} (lhs.[i] == ntt_kth_term (mul_quotient_ring f g) i));
+  // assert (forall (i:nat{i < n}).{:pattern (rhs.[i])} (rhs.[i] == (ntt f).[i] %* (ntt g).[i]));
+  assert (forall (i:nat{i < n}).{:pattern (lhs.[i]); (rhs.[i])} (lhs.[i] == rhs.[i]))
+
+
+val mul_ntt_ok:
+    f:rq
+  -> g:rq
+  -> Lemma 
+      (requires True) 
+      (ensures Seq.equal 
+        (mul_quotient_ring f g) 
+        (intt (mul_componentwise (ntt f) (ntt g))))
+let mul_ntt_ok f g =
+  convolution_theorem f g;
+  assert (Seq.equal
+            (intt (ntt (mul_quotient_ring f g))) 
+            (intt (mul_componentwise (ntt f) (ntt g))));
+  intt_ntt_is_id (mul_quotient_ring f g);
+  assert (mul_quotient_ring f g == intt (mul_componentwise (ntt f) (ntt g)))
+  
+
+
+// val ntt_inner_inner:
 //     z:zq
 //   -> f:tq
+//   -> j:nat
 //   -> len:len_t
 //   -> start:start_t len
-//   -> Lemma (ensures ntt_inner_inner z f start len start = ntt_inner_inner_func z f len start)
-// let ntt_inner_inner_func_ok z f len start = ()
+//   -> Tot (tq) (decreases (start + len) - j)
+// let rec ntt_inner_inner z f j len start: tq =
+//   // for j <- start; j < start + len; j++
+//   if j < (start + len) then
+//     // t <- zeta * f_hat[j+ len]
+//     let t = mul_zq z (index_tq f (j + len)) in
+//     let f_j = index_tq f j in
+//     // f_hat[j + len] <- f_hat[j] - t
+//     let f_upd = upd_tq f (j + len) (add_zq f_j (neg_zq t)) in
+//     // f_hat[j] <- f_hat[j] + t
+//     let f_upd_upd = upd_tq f_upd j (add_zq f_j t) in
+//     ntt_inner_inner z f_upd_upd (j + 1) len start
+//   else
+//     f
 
-val zeta_to_k:
-    k:nat{k < 128}
-  -> zq
-let zeta_to_k k = pow_mod #q zeta k
-let test = 
-  let zeta_0 = pow_mod #q zeta 0 in
-  pow_mod_def #q zeta 0;
-  lemma_pow_mod #q zeta 0;
-  lemma_pow0 zeta;
-  assert (zeta_0 = 1);
-  ()
+// val ntt_inner_inner_f (j:nat{j < 256}) (len:len_t) (start:start_t len) (z:zq) (f:tq): zq
+// let ntt_inner_inner_f j len start z f =
+//     if j < start || j >= start + 2 * len then
+//       index_tq f j
+//     else if j >= start && j < start + len then
+//       let t = mul_zq z (index_tq f (j + len)) in
+//       add_zq (index_tq f j) t
+//     else
+//       let t = mul_zq z (index_tq f j) in
+//       add_zq (index_tq f (j - len)) (neg_zq t)
 
-val zeta_to_k_pos_lemma: (k:nat{k > 0 && k < 128}) -> Lemma (requires True) (ensures (zeta_to_k k = mul_zq (zeta_to_k (k - 1)) zeta))
-let zeta_to_k_pos_lemma k = 
-  pow_mod_def #q zeta k;
-  lemma_pow_mod #q zeta k;
-  lemma_pow_unfold zeta k;
-  assert (pow zeta k % q = zeta_to_k k);
-  assert (zeta * pow zeta (k - 1) % q = zeta_to_k k);
-  lemma_pow_mod #q zeta (k - 1);
-  assert (pow zeta (k - 1) % q = zeta_to_k (k - 1));
-  ()
 
-val ntt_outer_inner_body:
-    f:tq
-  -> len:len_t
-  -> start:start_t len
-  -> k:nat{k < 128}
-  -> tq
-let ntt_outer_inner_body f len start k = 
-  // zeta <- Zeta ^ (BitRev7(k)) mod q
-  let z = pow_mod #q zeta (bitrev7_int k) in
-  let f_upd = ntt_inner_inner z f start len start in
-  f_upd
+// val ntt_inner_inner_func:
+//     z:zq 
+//   -> f:tq 
+//   -> len:len_t
+//   -> start:start_t len
+//   -> tq
+// let ntt_inner_inner_func z f len start = 
+//   let rq_rep = createi #zq 256 (fun j -> ntt_inner_inner_f j len start z f) in rq_to_tq rq_rep
 
-val ntt_outer_inner:
-    f:tq
-  -> len:len_t
-  -> start:start_t len
-  -> Tot (tq) (decreases (256 - 2 * len) - start)
-let rec ntt_outer_inner f len start =
-  let k = (128 / len) + (start / (2 * len)) in
-  let f_upd:tq = ntt_outer_inner_body f len start k in
-  if start + 2 * len >= 256 then 
-    f_upd
-  else
-    ntt_outer_inner f_upd len (start + 2 * len)
+// // val ntt_inner_inner_func_ok: 
+// //     z:zq
+// //   -> f:tq
+// //   -> len:len_t
+// //   -> start:start_t len
+// //   -> Lemma (ensures ntt_inner_inner z f start len start = ntt_inner_inner_func z f len start)
+// // let ntt_inner_inner_func_ok z f len start = ()
 
-val ntt_outer:
-    len:len_t
-  -> f:tq
-  -> Tot tq (decreases len)
-let rec ntt_outer len f =
-  let f_upd = ntt_outer_inner f len 0 in
-  if len = 2 then
-    f_upd
-  else
-    ntt_outer (len / 2) f_upd
-
-val len_t_lemma: (i:nat{i < 7}) -> 
-  Lemma (ensures pow2 i = 2 || pow2 i = 4 || pow2 i = 8 || pow2 i = 16 || pow2 i = 32 || pow2 i = 64)
-let len_t_lemma i = admit()
-
-val ntt_outer_intermediate:
-    f:tq
-  -> i:nat{i < 7}
-  -> Tot tq (decreases i)
-let rec ntt_outer_intermediate f i =
-  len_t_lemma (6-i);
-  let len:len_t = 128 / (pow2 (6-i)) in
-  let f_upd = ntt_outer_inner f len 0 in
-  if i = 0 then
-    f_upd
-  else
-    ntt_outer_intermediate f_upd (i-1)
-
-// val ntt_outer_int_ok: 
-//     f:tq
-//   -> Lemma (requires True) (ensures (ntt_outer 128 f = ntt_outer_intermediate f 6))
-// let ntt_outer_int_ok f =
-//   assert (ntt_outer 2 f = ntt_outer_intermediate f 0);
+// val zeta_to_k:
+//     k:nat{k < 128}
+//   -> zq
+// let zeta_to_k k = pow_mod #q zeta k
+// let test = 
+//   let zeta_0 = pow_mod #q zeta 0 in
+//   pow_mod_def #q zeta 0;
+//   lemma_pow_mod #q zeta 0;
+//   lemma_pow0 zeta;
+//   assert (zeta_0 = 1);
 //   ()
 
-let ntt (f:rq): tq =
-  let ntt_image = ntt_outer 128 (rq_to_tq f) in 
-  ntt_image
+// val zeta_to_k_pos_lemma: (k:nat{k > 0 && k < 128}) -> Lemma (requires True) (ensures (zeta_to_k k = mul_zq (zeta_to_k (k - 1)) zeta))
+// let zeta_to_k_pos_lemma k = 
+//   pow_mod_def #q zeta k;
+//   lemma_pow_mod #q zeta k;
+//   lemma_pow_unfold zeta k;
+//   assert (pow zeta k % q = zeta_to_k k);
+//   assert (zeta * pow zeta (k - 1) % q = zeta_to_k k);
+//   lemma_pow_mod #q zeta (k - 1);
+//   assert (pow zeta (k - 1) % q = zeta_to_k (k - 1));
+//   ()
 
-val intt_inner_inner:
-    z:zq
-  -> f:tq
-  -> j:nat
-  -> len:len_t
-  -> start:start_t len
-  -> Tot (tq) (decreases (start + len) - j)
-let rec intt_inner_inner z f j len start: tq =
-  // for j <- start; j < start + len; j++
-  if j < (start + len) then
-    // t <- zeta * f_hat[j+ len]
-    let t = (index_tq f j) in 
-    // f[j] <- t + f[j+len]
-    let f_j = add_zq t (index_tq f (j + len)) in
-    let f_upd = upd_tq f j f_j in
-    // f[j+len] <- zeta * (f[j+len] - t)
-    let f_j_len = mul_zq z (add_zq (index_tq f (j + len)) (neg_zq t)) in
-    let f_upd_upd = upd_tq f_upd (j + len) f_j_len in
-    intt_inner_inner z f_upd_upd (j + 1) len start
-  else
-    f
+// val ntt_outer_inner_body:
+//     f:tq
+//   -> len:len_t
+//   -> start:start_t len
+//   -> k:nat{k < 128}
+//   -> tq
+// let ntt_outer_inner_body f len start k = 
+//   // zeta <- Zeta ^ (BitRev7(k)) mod q
+//   let z = pow_mod #q zeta (bitrev7_int k) in
+//   let f_upd = ntt_inner_inner z f start len start in
+//   f_upd
 
-val intt_outer_inner_body:
-    f:tq
-  -> len:len_t
-  -> start:start_t len
-  -> k:nat{k < 128}
-  -> tq
-let intt_outer_inner_body f len start k =
-  // zeta <- Zeta ^ (BitRev7(k)) mod q
-  let z = pow_mod #q zeta (bitrev7_int k) in
-  let f_upd = intt_inner_inner z f start len start in
-  f_upd
+// val ntt_outer_inner:
+//     f:tq
+//   -> len:len_t
+//   -> start:start_t len
+//   -> Tot (tq) (decreases (256 - 2 * len) - start)
+// let rec ntt_outer_inner f len start =
+//   let k = (128 / len) + (start / (2 * len)) in
+//   let f_upd:tq = ntt_outer_inner_body f len start k in
+//   if start + 2 * len >= 256 then 
+//     f_upd
+//   else
+//     ntt_outer_inner f_upd len (start + 2 * len)
+
+// val ntt_outer:
+//     len:len_t
+//   -> f:tq
+//   -> Tot tq (decreases len)
+// let rec ntt_outer len f =
+//   let f_upd = ntt_outer_inner f len 0 in
+//   if len = 2 then
+//     f_upd
+//   else
+//     ntt_outer (len / 2) f_upd
+
+// val len_t_lemma: (i:nat{i < 7}) -> 
+//   Lemma (ensures pow2 i = 2 || pow2 i = 4 || pow2 i = 8 || pow2 i = 16 || pow2 i = 32 || pow2 i = 64)
+// let len_t_lemma i = admit()
+
+// val ntt_outer_intermediate:
+//     f:tq
+//   -> i:nat{i < 7}
+//   -> Tot tq (decreases i)
+// let rec ntt_outer_intermediate f i =
+//   len_t_lemma (6-i);
+//   let len:len_t = 128 / (pow2 (6-i)) in
+//   let f_upd = ntt_outer_inner f len 0 in
+//   if i = 0 then
+//     f_upd
+//   else
+//     ntt_outer_intermediate f_upd (i-1)
+
+// // val ntt_outer_int_ok: 
+// //     f:tq
+// //   -> Lemma (requires True) (ensures (ntt_outer 128 f = ntt_outer_intermediate f 6))
+// // let ntt_outer_int_ok f =
+// //   assert (ntt_outer 2 f = ntt_outer_intermediate f 0);
+// //   ()
+
+// let ntt (f:rq): tq =
+//   let ntt_image = ntt_outer 128 (rq_to_tq f) in 
+//   ntt_image
+
+// val intt_inner_inner:
+//     z:zq
+//   -> f:tq
+//   -> j:nat
+//   -> len:len_t
+//   -> start:start_t len
+//   -> Tot (tq) (decreases (start + len) - j)
+// let rec intt_inner_inner z f j len start: tq =
+//   // for j <- start; j < start + len; j++
+//   if j < (start + len) then
+//     // t <- zeta * f_hat[j+ len]
+//     let t = (index_tq f j) in 
+//     // f[j] <- t + f[j+len]
+//     let f_j = add_zq t (index_tq f (j + len)) in
+//     let f_upd = upd_tq f j f_j in
+//     // f[j+len] <- zeta * (f[j+len] - t)
+//     let f_j_len = mul_zq z (add_zq (index_tq f (j + len)) (neg_zq t)) in
+//     let f_upd_upd = upd_tq f_upd (j + len) f_j_len in
+//     intt_inner_inner z f_upd_upd (j + 1) len start
+//   else
+//     f
+
+// val intt_outer_inner_body:
+//     f:tq
+//   -> len:len_t
+//   -> start:start_t len
+//   -> k:nat{k < 128}
+//   -> tq
+// let intt_outer_inner_body f len start k =
+//   // zeta <- Zeta ^ (BitRev7(k)) mod q
+//   let z = pow_mod #q zeta (bitrev7_int k) in
+//   let f_upd = intt_inner_inner z f start len start in
+//   f_upd
 
 
-val intt_outer_inner:
-    f:tq
-  -> len:len_t
-  -> start:start_t len
-  -> Tot tq (decreases (256 - 2 * len) - start)
-let rec intt_outer_inner f len start =
-  let k = (256 / len) - (start / (2 * len)) - 1 in
-  // zeta <- Zeta ^ (BitRev7(k)) mod q
-  let z = pow_mod #q zeta (bitrev7_int k) in
-  let f_upd = intt_outer_inner_body f len start k in
-  if start + 2 * len >= 256 then
-    f_upd
-  else
-    intt_outer_inner f_upd len (start + 2 * len)
+// val intt_outer_inner:
+//     f:tq
+//   -> len:len_t
+//   -> start:start_t len
+//   -> Tot tq (decreases (256 - 2 * len) - start)
+// let rec intt_outer_inner f len start =
+//   let k = (256 / len) - (start / (2 * len)) - 1 in
+//   // zeta <- Zeta ^ (BitRev7(k)) mod q
+//   let z = pow_mod #q zeta (bitrev7_int k) in
+//   let f_upd = intt_outer_inner_body f len start k in
+//   if start + 2 * len >= 256 then
+//     f_upd
+//   else
+//     intt_outer_inner f_upd len (start + 2 * len)
 
-val intt_outer:
-    len:len_t
-  -> f:tq
-  -> Tot tq (decreases (128 - len))
-let rec intt_outer len f =
-  let f_upd = intt_outer_inner f len 0 in
-  if len = 128 then
-    f_upd
-  else
-    intt_outer (len * 2) f_upd
+// val intt_outer:
+//     len:len_t
+//   -> f:tq
+//   -> Tot tq (decreases (128 - len))
+// let rec intt_outer len f =
+//   let f_upd = intt_outer_inner f len 0 in
+//   if len = 128 then
+//     f_upd
+//   else
+//     intt_outer (len * 2) f_upd
 
-val intt:
-    f:tq
-  -> rq
-let intt f =
-  let intt_image = intt_outer 128 f in 
-  let unscaled_intt = tq_to_rq intt_image in
-  scalar_mul unscaled_intt 3303
+// val intt:
+//     f:tq
+//   -> rq
+// let intt f =
+//   let intt_image = intt_outer 128 f in 
+//   let unscaled_intt = tq_to_rq intt_image in
+//   scalar_mul unscaled_intt 3303
 
-// NTT multiplication specification
-// i-th coordinate in Tq of the product hat(h) = hat(f) x_Tq hat(g) is given by:
-//    hat(h)[2i] + hat(h)[2i+1] = (hat(f)[2i]+hat(f)[2i+1]X) * (hat(g)[2i]+hat(g)[2i+1]X) mod (X^2 - zeta^(2 BitRev_7(i)+1))
+// // NTT multiplication specification
+// // i-th coordinate in Tq of the product hat(h) = hat(f) x_Tq hat(g) is given by:
+// //    hat(h)[2i] + hat(h)[2i+1] = (hat(f)[2i]+hat(f)[2i+1]X) * (hat(g)[2i]+hat(g)[2i+1]X) mod (X^2 - zeta^(2 BitRev_7(i)+1))
 
-// index f i should yield an lpoly 2 which is equivalent to f[2i]+f[2i+1]X
-// ntt_mul_base calculates the product of two lpoly 2 with modulus X^2 - gamma
-let ntt_mul_base (a b:lpoly 2) (gamma: zq): lpoly 2 =
-  let c0 = add_zq (mul_zq (index a 0) (index b 0)) (mul_zq gamma (mul_zq (index a 1) (index b 1))) in
-  let c1 = add_zq (mul_zq (index a 0) (index b 1)) (mul_zq (index a 1) (index b 0)) in
-  cons c0 (cons c1 empty)
+// // index f i should yield an lpoly 2 which is equivalent to f[2i]+f[2i+1]X
+// // ntt_mul_base calculates the product of two lpoly 2 with modulus X^2 - gamma
+// let ntt_mul_base (a b:lpoly 2) (gamma: zq): lpoly 2 =
+//   let c0 = add_zq (mul_zq (index a 0) (index b 0)) (mul_zq gamma (mul_zq (index a 1) (index b 1))) in
+//   let c1 = add_zq (mul_zq (index a 0) (index b 1)) (mul_zq (index a 1) (index b 0)) in
+//   cons c0 (cons c1 empty)
